TFTP_Proofs.v
@@ -72,34 +72,153 @@ Theorem N_2b_correctness3 : forall x:N, forall p:string, forall s:string, String
       apply N_2b_correctness2.
       apply H0.
 Qed.
+
+Theorem ErrorCodeSerializationCorrectness : forall e:ErrorCode, DeserializeErrorCode (SerializeErrorCode e) = Some e.
+  intros.
+  induction e; simpl; trivial.
+Qed.
+Local Open Scope N_scope.
+Theorem ErrorCodeIsSmall : forall e:ErrorCode, SerializeErrorCode e < 256*256.
+  intros.
+  induction e; simpl; zify; omega.
+Qed.
+
 Lemma ParseNullTerminatedStringCorrectness : forall pref : string, forall rest : string, ParseNullTerminatedString (pref ++ String zero rest) = Some (pref, rest).
   admit.
 
 Admitted.
 
-Theorem SerializationCorrectness : forall m : TFTPMessage, Deserialize (Serialize m) = Some m.
-  intros.
-  induction m; unfold Serialize; unfold Deserialize.
-  * simpl. unfold OptBind.
-    rewrite -> ParseNullTerminatedStringCorrectness.
-    simpl.
-    trivial.
-  * simpl. unfold OptBind.
-    rewrite -> ParseNullTerminatedStringCorrectness.
-    simpl.
-    trivial.
-  * unfold OptBind.
-    assert (null = String zero EmptyString).
-  - auto.
-  - rewrite -> H.
-    simpl.
-    rewrite -> ParseNullTerminatedStringCorrectness.
-    simpl.
-    repeat f_equal.
-    repeat rewrite -> N_ascii_embedding.
-    zify. admit.
+Lemma ParseNullTerminatedStringCorrectness2 : forall pref : string, ParseNullTerminatedString (pref ++ null) = Some (pref, EmptyString).
+  admit.
+
+Admitted.
+
+(* We cannot prove serialization at once, because as for DATA and ACK it works only for messages that contain integers <= 65535 and the general datatype doesn't provide that, instead we'll prove specific instances *)
+(* Theorem SerializationCorrectness : forall m : TFTPMessage, Deserialize (Serialize m) = Some m. *)
+(*   intros. *)
+(*   induction m; unfold Serialize; unfold Deserialize. *)
+(*   * simpl. unfold OptBind. *)
+(*     rewrite -> ParseNullTerminatedStringCorrectness. *)
+(*     simpl. *)
+(*     trivial. *)
+(*   * simpl. unfold OptBind. *)
+(*     rewrite -> ParseNullTerminatedStringCorrectness. *)
+(*     simpl. *)
+(*     trivial. *)
+(*   * unfold OptBind. *)
+(*     assert (null = String zero EmptyString). *)
+(*   - auto. *)
+(*   - rewrite -> H. *)
+(*     simpl. *)
+(*     rewrite -> ParseNullTerminatedStringCorrectness. *)
+(*     simpl. *)
+(*     repeat f_equal. *)
+(*     repeat rewrite -> N_ascii_embedding. *)
+(*     zify. admit. *)
 
     
   
-  admit.
-Admitted. (* TODO *)
+(*   admit. *)
+(* Admitted. (* TODO *) *)
+
+(* Inductive TFTPMessage : Set *)
+(*   := RRQ (filename : string) *)
+(*    | WRQ (filename : string) *)
+(*    | ERROR (code : ErrorCode) (message : string) *)
+(*    | DATA (block : N) (data : string) *)
+(*    | ACK (block : N). *)
+Theorem SerializationCorrectness1 : forall f : string, Deserialize (Serialize (RRQ f)) = Some (RRQ f).
+  intros.
+  unfold Serialize; unfold Deserialize.
+  simpl.
+  unfold OptBind.
+  rewrite -> ParseNullTerminatedStringCorrectness.
+  simpl.
+  trivial.
+Qed.
+
+Theorem SerializationCorrectness2 : forall f : string, Deserialize (Serialize (WRQ f)) = Some (WRQ f).
+  intros.
+  unfold Serialize; unfold Deserialize.
+  simpl.
+  unfold OptBind.
+  rewrite -> ParseNullTerminatedStringCorrectness.
+  simpl.
+  trivial.
+Qed.
+
+Definition f (x : N) : N := match x
+           with
+           | 0 => 0
+           | N.pos q => N.pos q~0~0~0~0~0~0~0~0
+                            end.
+
+Compute f 4.
+
+Lemma N_rev_mul : forall x:N,
+    (match x with
+     | 0 => 0
+     | N.pos q => N.pos q~0~0~0~0~0~0~0~0
+     end) = 256 * x.
+  intros.
+  simpl.
+  trivial.
+Qed.
+
+Lemma N_2b_correctness4 : forall x: N,
+    (match x / 256 with
+     | 0 => 0
+     | N.pos q => N.pos q~0~0~0~0~0~0~0~0
+     end + x mod 256) = x.
+  intros.
+  rewrite -> N_rev_mul.
+  rewrite -> N.mod_eq.
+  remember (256 * (x / 256)) as a.
+  assert (a <= x).
+  * subst a.
+    apply N.mul_div_le.
+    zify; omega.
+  * zify; omega.
+  * zify; omega.
+Qed.
+
+Lemma PNTS_rev : forall s:string, (parseNullTerminatedHelper s []) = ParseNullTerminatedString s.
+  unfold ParseNullTerminatedString.
+  trivial.
+Qed.
+
+Lemma div_lemma1 : forall q:N, q < 256 * 256 -> q / 256 < 256.
+  intros.
+    assert (q <= 256 * 256 - 1).
+    ** zify; omega.
+    ** assert (q / 256 <= 255).
+       *** assert ((256 * 256 - 1) / 256 <= 255).
+  - simpl. unfold N.div. simpl. zify. omega.
+  - assert (q / 256 <= (256 * 256 - 1) / 256).
+    -- apply N.div_le_mono.
+       zify; omega. trivial.
+    -- rewrite <- H2. zify; omega.
+       *** zify; omega.
+Qed.
+Theorem SerializationCorrectness3 : forall c:ErrorCode, forall m:string, Deserialize (Serialize (ERROR c m)) = Some (ERROR c m).
+  intros.
+  unfold Serialize; unfold Deserialize.
+  unfold OptBind.
+  cbn.
+  repeat rewrite -> N_ascii_embedding.
+  rewrite -> N_2b_correctness4.
+  rewrite -> ErrorCodeSerializationCorrectness.
+  rewrite -> PNTS_rev.
+  rewrite -> ParseNullTerminatedStringCorrectness2.
+  simpl.
+  trivial.
+
+  apply N.mod_upper_bound.
+  zify;omega.
+
+  assert (SerializeErrorCode c < 256 * 256).
+  * apply ErrorCodeIsSmall.
+  * remember (SerializeErrorCode c) as q.
+    destruct Heqq.
+    apply div_lemma1. assumption.
+Qed.
